build/ir/Cdclt/Lift/Env.c
@@ -1,0 +1,203 @@
+// Lean compiler output
+// Module: Cdclt.Lift.Env
+// Imports: Init Cdclt.Lift.Types Cdclt.Lift.Coe Cdclt.Term
+#include <lean/lean.h>
+#if defined(__clang__)
+#pragma clang diagnostic ignored "-Wunused-parameter"
+#pragma clang diagnostic ignored "-Wunused-label"
+#elif defined(__GNUC__) && !defined(__CLANG__)
+#pragma GCC diagnostic ignored "-Wunused-parameter"
+#pragma GCC diagnostic ignored "-Wunused-label"
+#pragma GCC diagnostic ignored "-Wunused-but-set-variable"
+#endif
+#ifdef __cplusplus
+extern "C" {
+#endif
+LEAN_EXPORT lean_object* l_defaultSEnvironment___boxed(lean_object*);
+LEAN_EXPORT lean_object* l_defaultSEnvironment(lean_object*);
+static lean_object* l_defaultSEnvironment___closed__1;
+lean_object* lean_nat_add(lean_object*, lean_object*);
+LEAN_EXPORT lean_object* l_defaultEnvironment___rarg(lean_object*, lean_object*);
+uint8_t lean_nat_dec_eq(lean_object*, lean_object*);
+lean_object* lean_nat_sub(lean_object*, lean_object*);
+LEAN_EXPORT lean_object* l_defaultEnvironment___boxed(lean_object*);
+LEAN_EXPORT lean_object* l_defaultEnvironment(lean_object*);
+LEAN_EXPORT lean_object* l_defaultValue(lean_object*, lean_object*);
+LEAN_EXPORT lean_object* l_defaultValue___lambda__1(lean_object*, lean_object*, lean_object*);
+LEAN_EXPORT lean_object* l_defaultValue___lambda__1___boxed(lean_object*, lean_object*, lean_object*);
+static lean_object* _init_l_defaultSEnvironment___closed__1() {
+_start:
+{
+lean_object* x_1; lean_object* x_2; 
+x_1 = lean_unsigned_to_nat(0u);
+x_2 = lean_alloc_ctor(0, 2, 0);
+lean_ctor_set(x_2, 0, lean_box(0));
+lean_ctor_set(x_2, 1, x_1);
+return x_2;
+}
+}
+LEAN_EXPORT lean_object* l_defaultSEnvironment(lean_object* x_1) {
+_start:
+{
+lean_object* x_2; 
+x_2 = l_defaultSEnvironment___closed__1;
+return x_2;
+}
+}
+LEAN_EXPORT lean_object* l_defaultSEnvironment___boxed(lean_object* x_1) {
+_start:
+{
+lean_object* x_2; 
+x_2 = l_defaultSEnvironment(x_1);
+lean_dec(x_1);
+return x_2;
+}
+}
+LEAN_EXPORT lean_object* l_defaultValue___lambda__1(lean_object* x_1, lean_object* x_2, lean_object* x_3) {
+_start:
+{
+lean_object* x_4; 
+x_4 = l_defaultValue(x_1, x_2);
+return x_4;
+}
+}
+LEAN_EXPORT lean_object* l_defaultValue(lean_object* x_1, lean_object* x_2) {
+_start:
+{
+switch (lean_obj_tag(x_2)) {
+case 1:
+{
+lean_object* x_3; lean_object* x_4; uint8_t x_5; 
+x_3 = lean_ctor_get(x_2, 0);
+lean_inc(x_3);
+lean_dec(x_2);
+x_4 = lean_unsigned_to_nat(0u);
+x_5 = lean_nat_dec_eq(x_3, x_4);
+if (x_5 == 0)
+{
+lean_object* x_6; lean_object* x_7; uint8_t x_8; 
+x_6 = lean_unsigned_to_nat(1u);
+x_7 = lean_nat_sub(x_3, x_6);
+lean_dec(x_3);
+x_8 = lean_nat_dec_eq(x_7, x_4);
+if (x_8 == 0)
+{
+lean_object* x_9; lean_object* x_10; lean_object* x_11; lean_object* x_12; lean_object* x_13; 
+x_9 = lean_nat_sub(x_7, x_6);
+lean_dec(x_7);
+x_10 = lean_nat_add(x_9, x_6);
+lean_dec(x_9);
+x_11 = lean_nat_add(x_10, x_6);
+lean_dec(x_10);
+x_12 = lean_apply_1(x_1, x_11);
+x_13 = lean_ctor_get(x_12, 1);
+lean_inc(x_13);
+lean_dec(x_12);
+return x_13;
+}
+else
+{
+uint8_t x_14; lean_object* x_15; 
+lean_dec(x_7);
+lean_dec(x_1);
+x_14 = 0;
+x_15 = lean_box(x_14);
+return x_15;
+}
+}
+else
+{
+lean_object* x_16; lean_object* x_17; 
+lean_dec(x_3);
+x_16 = lean_apply_1(x_1, x_4);
+x_17 = lean_ctor_get(x_16, 1);
+lean_inc(x_17);
+lean_dec(x_16);
+return x_17;
+}
+}
+case 2:
+{
+lean_object* x_18; lean_object* x_19; 
+x_18 = lean_ctor_get(x_2, 1);
+lean_inc(x_18);
+lean_dec(x_2);
+x_19 = lean_alloc_closure((void*)(l_defaultValue___lambda__1___boxed), 3, 2);
+lean_closure_set(x_19, 0, x_1);
+lean_closure_set(x_19, 1, x_18);
+return x_19;
+}
+default: 
+{
+uint8_t x_20; lean_object* x_21; 
+lean_dec(x_2);
+lean_dec(x_1);
+x_20 = 0;
+x_21 = lean_box(x_20);
+return x_21;
+}
+}
+}
+}
+LEAN_EXPORT lean_object* l_defaultValue___lambda__1___boxed(lean_object* x_1, lean_object* x_2, lean_object* x_3) {
+_start:
+{
+lean_object* x_4; 
+x_4 = l_defaultValue___lambda__1(x_1, x_2, x_3);
+lean_dec(x_3);
+return x_4;
+}
+}
+LEAN_EXPORT lean_object* l_defaultEnvironment___rarg(lean_object* x_1, lean_object* x_2) {
+_start:
+{
+lean_object* x_3; 
+x_3 = l_defaultValue(x_1, x_2);
+return x_3;
+}
+}
+LEAN_EXPORT lean_object* l_defaultEnvironment(lean_object* x_1) {
+_start:
+{
+lean_object* x_2; 
+x_2 = lean_alloc_closure((void*)(l_defaultEnvironment___rarg), 2, 0);
+return x_2;
+}
+}
+LEAN_EXPORT lean_object* l_defaultEnvironment___boxed(lean_object* x_1) {
+_start:
+{
+lean_object* x_2; 
+x_2 = l_defaultEnvironment(x_1);
+lean_dec(x_1);
+return x_2;
+}
+}
+lean_object* initialize_Init(uint8_t builtin, lean_object*);
+lean_object* initialize_Cdclt_Lift_Types(uint8_t builtin, lean_object*);
+lean_object* initialize_Cdclt_Lift_Coe(uint8_t builtin, lean_object*);
+lean_object* initialize_Cdclt_Term(uint8_t builtin, lean_object*);
+static bool _G_initialized = false;
+LEAN_EXPORT lean_object* initialize_Cdclt_Lift_Env(uint8_t builtin, lean_object* w) {
+lean_object * res;
+if (_G_initialized) return lean_io_result_mk_ok(lean_box(0));
+_G_initialized = true;
+res = initialize_Init(builtin, lean_io_mk_world());
+if (lean_io_result_is_error(res)) return res;
+lean_dec_ref(res);
+res = initialize_Cdclt_Lift_Types(builtin, lean_io_mk_world());
+if (lean_io_result_is_error(res)) return res;
+lean_dec_ref(res);
+res = initialize_Cdclt_Lift_Coe(builtin, lean_io_mk_world());
+if (lean_io_result_is_error(res)) return res;
+lean_dec_ref(res);
+res = initialize_Cdclt_Term(builtin, lean_io_mk_world());
+if (lean_io_result_is_error(res)) return res;
+lean_dec_ref(res);
+l_defaultSEnvironment___closed__1 = _init_l_defaultSEnvironment___closed__1();
+lean_mark_persistent(l_defaultSEnvironment___closed__1);
+return lean_io_result_mk_ok(lean_box(0));
+}
+#ifdef __cplusplus
+}
+#endif
